More progress on compile_well_typed_unaryApp
Signed-off-by: Zhengyao Lin <zyal@amazon.com>

cedar-lean/Cedar/Thm/SymCC/Compiler/WellTyped.lean
@@ -14,25 +14,38 @@ States that under sufficiently good conditions, the symbolic compiler
 succeeds on a typed expression `ty` and produces a term `t` with the
 corresponding type.
 -/
-def CompileWellTypedResult (ty : TypedExpr) (εnv : SymEnv) : Prop :=
+def CompileWellTypedForExpr (ty : TypedExpr) (εnv : SymEnv) : Prop :=
   ∃ t : Term,
     compile ty.toExpr εnv = .ok t ∧
     t.typeOf = .option (TermType.ofType ty.typeOf)
 
-def CompileWellTyped (ty : TypedExpr) (env : Environment) (εnv : SymEnv) : Prop :=
-  εnv = SymEnv.ofEnv env →
-  TypedExpr.WellTyped env ty →
-  εnv.WellFormedFor ty.toExpr →
-  CompileWellTypedResult ty εnv
+def CompileWellTypedCondition (ty : TypedExpr) (env : Environment) (εnv : SymEnv) : Prop :=
+  εnv = SymEnv.ofEnv env ∧
+  TypedExpr.WellTyped env ty ∧
+  εnv.WellFormedFor ty.toExpr
+
+/--
+A wrapper around compile_wf for convenience
+-/
+theorem CompileWellTypedCondition_implies_compile_well_formed
+  {ty : TypedExpr} {env : Environment} {εnv : SymEnv} {t : Term} :
+  CompileWellTypedCondition ty env εnv →
+  compile ty.toExpr εnv = .ok t →
+  t.WellFormed εnv.entities
+:= by
+  intros h hcomp; rcases h with ⟨henv, hwt, hwf⟩
+  have htwf := compile_wf hwf hcomp
+  simp [htwf]
 
 /--
 Special case for literals
 -/
 theorem compile_well_typed_lit {p : Prim} {ty : CedarType} {env : Environment} {εnv : SymEnv} :
-  CompileWellTyped (.lit p ty) env εnv
+  CompileWellTypedCondition (.lit p ty) env εnv →
+  CompileWellTypedForExpr (.lit p ty) εnv
 := by
-  intros henv hwt hwf
-  simp [TypedExpr.typeOf, TypedExpr.toExpr, CompileWellTypedResult] at *
+  intros h; rcases h with ⟨henv, hwt, hwf⟩
+  simp [TypedExpr.typeOf, TypedExpr.toExpr, CompileWellTypedForExpr] at *
 
   unfold SymEnv.WellFormedFor at hwf
   rcases hwf with ⟨_, ⟨hrefs⟩⟩
@@ -125,10 +138,11 @@ theorem isCedarRecordType_implies_isRecordType
 
 /- Special case for variables -/
 theorem compile_well_typed_var {v : Var} {ty : CedarType} {env : Environment} {εnv : SymEnv} :
-  CompileWellTyped (.var v ty) env εnv
+  CompileWellTypedCondition (.var v ty) env εnv →
+  CompileWellTypedForExpr (.var v ty) εnv
 := by
-  intros henv hwt hwf
-  simp [TypedExpr.typeOf, TypedExpr.toExpr, CompileWellTypedResult] at *
+  intros h; rcases h with ⟨henv, hwt, hwf⟩
+  simp [TypedExpr.typeOf, TypedExpr.toExpr, CompileWellTypedForExpr] at *
 
   unfold SymEnv.WellFormedFor SymEnv.WellFormed SymRequest.WellFormed at hwf
 
@@ -166,181 +180,224 @@ theorem compile_well_typed_var {v : Var} {ty : CedarType} {env : Environment} {�
     simp [TermType.ofType, Term.typeOf]
     simp [henv, SymEnv.ofEnv, SymRequest.ofRequestType, TermType.ofType, TermPrim.typeOf, Term.typeOf]
 
+theorem wf_typeOf_ite {g t₁ t₂ : Term} {ty : TermType} {entities : SymEntities}
+  (hwf_g : g.WellFormed entities)
+  (hwf_t1 : t₁.WellFormed entities)
+  (hwf_t2 : t₂.WellFormed entities)
+  (hbool_g : g.typeOf = TermType.bool)
+  (htyeq1 : t₁.typeOf = ty)
+  (htyeq2 : t₂.typeOf = ty) :
+  (Factory.ite g t₁ t₂).typeOf = ty
+:= by
+  have h1 : t₁.typeOf = t₂.typeOf := by simp [htyeq1, htyeq2]
+  have h := wf_ite hwf_g hwf_t1 hwf_t2 hbool_g h1
+  rw [h.right]; assumption
+
+theorem wf_typeOf_not {t : Term} {ty : TermType} {entities : SymEntities}
+  (hwf : t.WellFormed entities)
+  (hbool_t : t.typeOf = ty)
+  (hty : ty = .bool) :
+  (Factory.not t).typeOf = ty
+:= by
+  have h1 : t.typeOf = .bool := by simp [hbool_t, hty]
+  have h := wf_not hwf h1
+  rw [h.right]; simp [hty]
+
 mutual
   theorem compile_well_typed_ite
     {cond : TypedExpr} {thenExpr : TypedExpr} {elseExpr : TypedExpr} {ty : CedarType}
     {env : Environment} {εnv : SymEnv}:
-    CompileWellTyped (.ite cond thenExpr elseExpr ty) env εnv
+    CompileWellTypedCondition (.ite cond thenExpr elseExpr ty) env εnv →
+    CompileWellTypedForExpr (.ite cond thenExpr elseExpr ty) εnv
   := by
-    intros henv hwt hwf
-    simp [TypedExpr.typeOf, TypedExpr.toExpr] at *
+    intros h; rcases h with ⟨henv, hwt, hwf⟩
+    simp [TypedExpr.typeOf, TypedExpr.toExpr, CompileWellTypedForExpr] at *
     sorry
 
   theorem compile_well_typed_and
     {a : TypedExpr} {b : TypedExpr} {ty : CedarType}
-    {env : Environment} {εnv : SymEnv} :
-    CompileWellTypedResult a εnv →
-    CompileWellTypedResult b εnv →
-    CompileWellTyped (.and a b ty) env εnv
+    {env : Environment} {εnv : SymEnv}
+    (iha: CompileWellTypedForExpr a εnv)
+    (ihb : CompileWellTypedForExpr b εnv)
+    (hcond_and : CompileWellTypedCondition (.and a b ty) env εnv) :
+    CompileWellTypedForExpr (.and a b ty) εnv
   := by
-    intros ha hb henv hwt hwf
-    simp [CompileWellTypedResult] at *
+    -- Some facts needed later
+    have ⟨hcond_a, hcond_b⟩ := CompileWellTypedCondition_and hcond_and
+    have ⟨henv, hwt_and, hwf_and⟩ := hcond_and
 
-    let ⟨t_a, ⟨hcomp_a, hty_a⟩⟩ := ha
-    let ⟨t_b, ⟨hcomp_b, hty_b⟩⟩ := hb
+    have ⟨tcomp_a, ⟨hcomp_a, hty_comp_a⟩⟩ := iha
+    have ⟨tcomp_b, ⟨hcomp_b, hty_comp_b⟩⟩ := ihb
+
+    have hwf_comp_a := CompileWellTypedCondition_implies_compile_well_formed hcond_a hcomp_a
+    have hwf_comp_b := CompileWellTypedCondition_implies_compile_well_formed hcond_b hcomp_b
+
+    have ⟨hwf_get_comp_a, hty_get_comp_a⟩ := wf_option_get hwf_comp_a hty_comp_a
+    have ⟨hwf_get_comp_b, hty_get_comp_b⟩ := wf_option_get hwf_comp_b hty_comp_b
 
     -- By well-typedness, a and b must be booleans
-    cases hwt
-    case and _ hbool_a _ hbool_b =>
+    -- So we substitute that fact and simplify
+    cases hwt_and; case and _ hbool_a _ hbool_b =>
+    simp [hbool_a, hbool_b] at *; clear hbool_a hbool_b
+    simp [TypedExpr.typeOf, TermType.ofType] at *
 
-    simp [compile, compileAnd, TypedExpr.typeOf, TypedExpr.toExpr] at *
     simp [
-      hcomp_a, hcomp_b, hty_a, hty_b, hbool_a, hbool_b,
-      TermType.ofType, Term.typeOf,
+      CompileWellTypedForExpr,
+      TypedExpr.toExpr,
+      compile,
+      compileAnd,
+      hcomp_a, hty_comp_a, hcomp_b, hty_comp_b,
+    ]
+    split
+    · apply Exists.intro; constructor; rfl
+      simp [Term.typeOf, TermPrim.typeOf, TermType.ofType, TypedExpr.typeOf]
+    · apply Exists.intro; constructor; rfl
+      apply typeOf_ifSome_option
+      apply wf_typeOf_ite
+      any_goals assumption
+      constructor
+      apply wf_bool
+      simp [TermType.ofType, Term.typeOf, TermPrim.typeOf, Factory.someOf, TypedExpr.typeOf]
+    · contradiction
+
+  /--
+  CompileWellTypedCondition decomposes for and
+  -/
+  theorem CompileWellTypedCondition_and {a : TypedExpr} {b : TypedExpr} {ty : CedarType} {env : Environment} {εnv : SymEnv} :
+    CompileWellTypedCondition (.and a b ty) env εnv →
+    CompileWellTypedCondition a env εnv ∧
+    CompileWellTypedCondition b env εnv
+  := by
+    intros h; rcases h with ⟨henv, hwt, hwf⟩
+    constructor
+    all_goals
+      constructor
+      any_goals assumption
+
+      constructor
+      · cases hwt; assumption
+      · simp [SymEnv.WellFormedFor, SymEntities.ValidRefsFor, TypedExpr.toExpr] at *
+        rcases hwf with ⟨_, hrefs⟩
+        constructor; assumption
+        cases hrefs; assumption
+
+  /--
+  CompileWellTypedCondition decomposes for unaryApp
+  -/
+  theorem CompileWellTypedCondition_unaryApp
+    {op : UnaryOp} {expr : TypedExpr} {ty : CedarType} {env : Environment} {εnv : SymEnv} :
+    CompileWellTypedCondition (.unaryApp op expr ty) env εnv →
+    CompileWellTypedCondition expr env εnv
+  := by
+    intros h; rcases h with ⟨henv, hwt, hwf⟩
+    constructor; any_goals assumption
+    constructor
+    · cases hwt; assumption
+    · simp [SymEnv.WellFormedFor, SymEntities.ValidRefsFor, TypedExpr.toExpr] at *
+      rcases hwf with ⟨_, hrefs⟩
+      constructor; assumption
+      cases hrefs; assumption
+
+  theorem compile_well_typed_unaryApp
+    {op : UnaryOp} {expr : TypedExpr} {ty : CedarType}
+    {env : Environment} {εnv : SymEnv}
+    (ihexpr : CompileWellTypedForExpr expr εnv)
+    (hcond_unary : CompileWellTypedCondition (.unaryApp op expr ty) env εnv) :
+    CompileWellTypedForExpr (.unaryApp op expr ty) εnv
+  := by
+    have hcond_expr := CompileWellTypedCondition_unaryApp hcond_unary
+    have ⟨henv, hwt, hwf⟩ := hcond_unary
+    have ⟨compile_expr, hcomp_expr, hty_comp_expr⟩ := ihexpr
+
+    have hwf_expr := CompileWellTypedCondition_implies_compile_well_formed hcond_expr hcomp_expr
+    have ⟨hwf_get_expr, hty_get_expr⟩ := wf_option_get hwf_expr hty_comp_expr
+
+    -- simp [CompileWellTypedForExpr, TypedExpr.toExpr] at *
+
+    -- Case analysis on the operator
+    cases hwt
+    case unaryApp _ hopwt =>
+    cases hopwt
+
+    -- Some simplification on all goals
+    all_goals simp [
+      CompileWellTypedForExpr,
+      hcomp_expr,
+      hty_get_expr,
+      TypedExpr.toExpr,
+      compile,
+      compileApp₁,
+      Term.typeOf,
     ]
 
-    split
-    · simp [Term.typeOf, TermPrim.typeOf]
-    · simp
+    case not hty_expr =>
+      simp [hty_expr, TermType.ofType] at hty_comp_expr
+      simp [hty_expr, TermType.ofType, Factory.someOf]
       rw [typeOf_ifSome_option]
-      rw [typeOf_ite]
-      rw [typeOf_option_get]
-      simp [hty_a, hbool_a, TermType.ofType]
-      simp [hty_b, hbool_b, TermType.ofType]
-      simp [Factory.someOf, TermType.ofType, Term.typeOf, TermPrim.typeOf]
+      simp [TypedExpr.typeOf, TermType.ofType, Term.typeOf]
 
-    · contradiction
+      apply wf_typeOf_not
+      any_goals assumption
+      any_goals simp
+
+      simp [hty_get_expr, hty_expr, TermType.ofType, Term.typeOf]
+
+    case neg hty_expr =>
+      simp [hty_expr, TermType.ofType] at hty_comp_expr hty_get_expr
+      simp [hty_expr, TermType.ofType, Factory.someOf]
+      rw [typeOf_ifSome_option]
+      simp [TypedExpr.typeOf, TermType.ofType, Term.typeOf, Factory.ifFalse, Factory.noneOf, Factory.someOf]
+
+      have ⟨hwf_bvnego_get_expr, hty_bvnego_get_expr⟩ := wf_bvnego hwf_get_expr hty_get_expr
+      have ⟨hwf_bvneg_get_expr, hty_bvneg_get_expr⟩ := wf_bvneg hwf_get_expr hty_get_expr
+
+      apply wf_typeOf_ite
+      any_goals assumption
+      any_goals simp [TermType.ofType, Term.typeOf, TermPrim.typeOf, Factory.someOf]
+
+      · constructor
+        simp [*]
+        constructor
+      · constructor; assumption
+      · simp [*]
+      · simp [*]
+
+    all_goals sorry
 
   /--
   Compiling a well-typed expression should produce a term of the corresponding TermType.
   -/
   theorem compile_well_typed {env : Environment} {εnv : SymEnv} {ty : TypedExpr} :
-    CompileWellTyped ty env εnv
+    CompileWellTypedCondition ty env εnv →
+    CompileWellTypedForExpr ty εnv
   := by
+    intros h
     cases ty
-    case lit => exact compile_well_typed_lit
-    case var => exact compile_well_typed_var
-    case ite => exact compile_well_typed_ite
+    case lit => exact compile_well_typed_lit h
+    case var => exact compile_well_typed_var h
+    case ite => exact compile_well_typed_ite h
     case and =>
-      intros henv hwt hwf
+      have ⟨ha, hb⟩ := CompileWellTypedCondition_and h
       apply compile_well_typed_and
-      any_goals assumption
+      any_goals apply compile_well_typed
+      all_goals assumption
 
-      -- Prove IH
-      all_goals
-        apply compile_well_typed
-        any_goals assumption
-        cases hwt
-        any_goals assumption
-        simp [SymEnv.WellFormedFor, SymEntities.ValidRefsFor] at *
-        rcases hwf with ⟨hwf, hrefs⟩
-        simp [Expr.ValidRefs, TypedExpr.toExpr] at hrefs
-        constructor; assumption
-        cases hrefs; assumption
+    case unaryApp =>
+      have hcond := CompileWellTypedCondition_unaryApp h
+      apply compile_well_typed_unaryApp
+      any_goals apply compile_well_typed
+      all_goals assumption
 
     all_goals sorry
-  -- termination_by (sizeOf ty)
 end
 
-  -- intros henv hwt hwf hcomp
-
-  -- unfold
-  --   SymEnv.WellFormedFor
-  --   SymEntities.ValidRefsFor
-  --   SymEnv.WellFormed
-  --   SymRequest.WellFormed at hwf
-
-  -- rcases hwf with ⟨⟨hreqwf, henvwf⟩, hrefs⟩
-  -- rcases hreqwf with ⟨
-  --   hreqwf₁,
-  --   hreqwf₂,
-  --   hreqwf₃,
-  --   hreqwf₄,
-  --   hreqwf₅,
-  --   hreqwf₆,
-  --   hreqwf₇,
-  --   hreqwf₈
-  -- ⟩
-
-  -- cases e : ty
-  -- all_goals
-  --   rw [e] at hcomp hwt hrefs
-  --   unfold TypedExpr.toExpr at hrefs
-  --   unfold compile TypedExpr.toExpr at hcomp
-  --   simp at *
-  --   -- unfold Factory.someOf Term.typeOf TermPrim.typeOf TypedExpr.typeOf TermType.ofType at *
-  --   -- cases hwt
-
-  -- case lit p =>
-  --   unfold compilePrim at hcomp
-  --   cases hwt
-  --   cases p
-
-  --   case entity =>
-  --     cases hrefs
-  --     case lit_valid hrefs =>
-  --       unfold Prim.ValidRef at hrefs
-  --       unfold Factory.someOf at hcomp
-  --       simp at *
-  --       rw [hrefs] at hcomp
-  --       simp at *
-  --       rw [←hcomp]
-  --       unfold Term.typeOf TermPrim.typeOf at *
-  --       simp
-
-  --   -- Other cases can be resolved by rewriting
-  --   any_goals
-  --     simp at *
-  --     rw [←hcomp]
-  --     unfold Term.typeOf TermPrim.typeOf BitVec.width at *
-  --     simp
-
-  -- case var v =>
-  --   cases v
-  --   all_goals
-  --     unfold compileVar at hcomp
-  --     simp at *
-
-  --   case principal =>
-
-  --     sorry
-
-  --   all_goals sorry
-
-  -- all_goals sorry
-
-  -- | lit p =>
-  --   sorry
-  -- | _ => sorry
-
-  -- let x := ty.toExpr
-  -- have h₄ : compile x εnv = .ok t := h₄
-  -- match x with
-  -- | .lit (.bool b) =>
-  --   -- unfold TypedExpr.typeOf
-  --   -- unfold compile compilePrim Factory.someOf at h₄
-  --   -- simp at h₄
-  --   -- unfold Term.typeOf TermPrim.typeOf
-  --   -- rw [←h₄]
-  --   -- simp
-  --   -- unfold Term.typeOf TermPrim.typeOf
-  --   -- simp
-  --   cases h₂ with
-  --   | lit p => sorry
-  --   | var v =>
-  --     cases v with
-  --     | principal => sorry
-  --     | _ => sorry
-  --   | _ => sorry
-  -- | _ => sorry
-
-theorem compile_well_typed_expr_never_fails {ty : TypedExpr} {env : Environment} {εnv : SymEnv} :
-  εnv = SymEnv.ofEnv env →
-  TypedExpr.WellTyped env ty →
-  εnv.WellFormedFor ty.toExpr →
-  Except.isOk (compile ty.toExpr εnv)
-:= by
-  intros
-  sorry
+-- theorem compile_well_typed_expr_never_fails {ty : TypedExpr} {env : Environment} {εnv : SymEnv} :
+--   εnv = SymEnv.ofEnv env →
+--   TypedExpr.WellTyped env ty →
+--   εnv.WellFormedFor ty.toExpr →
+--   Except.isOk (compile ty.toExpr εnv)
+-- := by
+--   intros
+--   sorry
 
 end Cedar.Thm
