cedar-lean/Cedar/Thm/SymCC/Term/TypeOf.lean
@@ -415,44 +415,22 @@ theorem typeOf_ifAllSome_option_type {gs : List Term} {t : Term} {ty : TermType}
   simp only [ifAllSome, hty, Factory.ite, noneOf]
   exact typeOf_ite_simplify_option hty
 
-theorem typeOf_not {t : Term} {ty : TermType} :
+theorem typeOf_not {t : Term} {entities : SymEntities} :
+  t.WellFormed entities →
   t.typeOf = TermType.bool →
   (not t).typeOf = TermType.bool
 := by
-  intro ht
+  intro hwf ht
   simp [Factory.not]
   split
   all_goals simp [Term.typeOf, TermPrim.typeOf] at *
-  -- TODO
-  all_goals sorry
 
-theorem typeOf_ite {g t₁ t₂ : Term} {ty : TermType} :
-  g.typeOf = TermType.bool →
-  t₁.typeOf = ty →
-  t₂.typeOf = ty →
-  (ite g t₁ t₂).typeOf = ty
-:= by
-  intros hg h₁ h₂
-  simp [Factory.ite, Factory.ite.simplify]
-  split; split
-  any_goals assumption
-  split
-  any_goals assumption
-  split
-  · simp [Term.typeOf, TermPrim.typeOf, hg] at *; assumption
-
-  · simp [Term.typeOf, TermPrim.typeOf, hg] at h₁
-    simp [Term.typeOf, TermPrim.typeOf, hg]
-    rw [typeOf_not]
-    all_goals assumption
-
-  -- TODO
-
-  all_goals sorry
-
-theorem typeOf_option_get {t : Term} {ty : TermType} :
-  t.typeOf = TermType.option ty →
-  (option.get t).typeOf = ty
-:= sorry
+  -- The last case is for `not (not t) => t`
+  -- which requires the well-formedness condition
+  cases hwf
+  case app_wf _ hopwf =>
+  cases hopwf
+  case not_wt htt =>
+  exact htt
 
 end Cedar.Thm
